src/type_directed_translation_tests.v
@@ -169,12 +169,14 @@ Proof.
       (TyArrDep "x" (TyBase BNat) (TyBase BNat)) surf_const_dep_fun_nat_expr).
     + unfold surf_impure_app_ctx, var_ctx_lookup_surf, ctx_add_var_surf. compute. reflexivity.
     + intro H.
+      specialize (H (TBase BNat)).
       inversion H; subst.
       destruct τb; simpl in *; try contradiction; discriminate.
   - simple eapply (@ATGet sim surf_impure_app_ctx (ExVar "r") (EVar "r") (TBase BNat)).
     simple eapply (@ATVar sim surf_impure_app_ctx "r" (TyRef (TyBase BNat)) (ExVar "r")).
     + unfold surf_impure_app_ctx, var_ctx_lookup_surf, ctx_add_var_surf. compute. reflexivity.
     + intro H.
+      specialize (H (TBase BNat)).
       inversion H; subst.
       destruct τb; simpl in *; try contradiction; discriminate.
   - apply CSub. apply SBase.
